WIP: simulation relation

theories/simulation.v
@@ -31,6 +31,7 @@ Definition sim_val_expr (e1 e2: expr) :=
    - cpro: Call states are the same
    - cstk: TODO missing relation between stacks
    - cclk: TODO missing relation between tag clocks *)
+(* TODO: alloc need to be deterministic *)
 Record sim_state (σ_src σ_tgt: state) := {
   sim_state_mem_dom : dom (gset loc) σ_src.(cheap) ≡ dom (gset loc) σ_tgt.(cheap);
   sim_state_stack_dom : dom (gset loc) σ_src.(cstk) ≡ dom (gset loc) σ_tgt.(cstk);
@@ -68,8 +69,11 @@ Qed.
 (* This is a simulation between two expressions without any interference.
   It corresponds to a sequential simulation. *)
 
-Notation SIM_EXPR := (relation expr)%type.
-Notation SIM_THREAD := (SIM_EXPR → expr → state → expr → state → Prop)%type.
+Notation SIM_CONFIG := (relation (expr * state))%type.
+Notation SIM_THREAD := (SIM_CONFIG → SIM_CONFIG)%type.
+
+Infix "~t~>" := thread_step (at level 70).
+Infix "~t~>*" := (rtc thread_step) (at level 70).
 
 (* Generator for the actual simulation *)
 (* TODO: sim_state is not right *)
@@ -83,126 +87,144 @@ Notation SIM_THREAD := (SIM_EXPR → expr → state → expr → state → Prop)
   The values can contain any observations of the states in between by reading
   the memory. Thus the simulation maintains the relation `sim_state` between
   the states. *)
-Definition _sim_thread (sim_thread: SIM_THREAD) (sim_terminal: SIM_EXPR)
-  (e1_src: expr) (σ1_src: state) (e1_tgt: expr) (σ1_tgt: state) : Prop :=
-  (* Wf ρ1_src → Wf ρ1_tgt → *)
-  Wf σ1_src → Wf σ1_tgt →
-  (* σ1_src, σ1_tgt are related *)
-  sim_state σ1_src σ1_tgt →
+Definition _sim_thread (sim_thread: SIM_THREAD) (sim_term: SIM_CONFIG)
+  (eσ1_src eσ1_tgt: expr * state) : Prop :=
+  Wf eσ1_src.2 → Wf eσ1_tgt.2 →
   (* (1) If `e1_tgt` is terminal, then `e1_src` terminates with τ steps *)
-  (terminal e1_tgt → ∃ e2_src σ2_src,
-    rtc thread_step (e1_src, σ1_src) (e2_src, σ2_src) ∧
-    sim_state σ2_src σ1_tgt ∧
-    terminal e2_src ∧ sim_terminal e2_src e1_tgt) ∧
+  (terminal eσ1_tgt.1 → ∃ eσ2_src,
+    eσ1_src ~t~>* eσ2_src ∧ terminal eσ2_src.1 ∧ sim_term eσ2_src eσ1_tgt) ∧
   (* (2) If `(e1_tgt, σ1_tgt)` steps to `(e2_tgt, σ2_tgt)` with 1+ step,
          then exists `(e2_src, σ2_src)`
          s.t. `(e1_src, σ1_src)` steps to `(e2_src, σ2_src)` with * step
          and still maintains the relation. *)
-  (∀ e2_tgt σ2_tgt, thread_step (e1_tgt, σ1_tgt) (e2_tgt, σ2_tgt) →
-      ∃ e2_src σ2_src,
-      rtc thread_step (e1_src, σ1_src) (e2_src, σ2_src) ∧
-      sim_state σ2_src σ2_tgt ∧
-      sim_thread sim_terminal e2_src σ2_src e2_tgt σ2_tgt).
+  (∀ eσ2_tgt, eσ1_tgt ~t~> eσ2_tgt → ∃ eσ2_src,
+      eσ1_src ~t~>* eσ2_src ∧ sim_thread sim_term eσ2_src eσ2_tgt).
 
-Lemma _sim_thread_mono : monotone5 _sim_thread.
+Lemma _sim_thread_mono : monotone3 _sim_thread.
 Proof.
-  intros re ???? r r' TS LE WF1 WF2 SS.
-  destruct (TS WF1 WF2 SS) as [TERM STEP]. split; [done|].
-  intros e2_tgt σ2_tgt ONE.
-  destruct (STEP _ _ ONE) as (e2_src & σ2_src & STEP1 & SS' & Hr).
-  exists e2_src, σ2_src. do 2 (split; [done|]). by apply LE.
+  intros re ?? r r' TS LE WF1 WF2.
+  destruct (TS WF1 WF2) as [TERM STEP]. split; [done|].
+  intros eσ2_tgt ONE. destruct (STEP _ ONE) as (eσ2_src & STEP1 & Hr).
+  exists eσ2_src. split; [done|]. by apply LE.
 Qed.
 Hint Resolve _sim_thread_mono: paco.
 
 (* Actual simulation *)
-Definition sim_thread: SIM_THREAD := paco5 _sim_thread bot5.
+Definition sim_thread: SIM_THREAD := paco3 _sim_thread bot3.
 
 Lemma thread_step_wf eσ1 eσ2 :
-  thread_step eσ1 eσ2 → Wf eσ1.2 → Wf eσ2.2.
+  eσ1 ~t~> eσ2 → Wf eσ1.2 → Wf eσ2.2.
 Proof. inversion 1. inversion PRIM. by eapply head_step_wf. Qed.
 Lemma rtc_thread_step_wf eσ1 eσ2 :
-  rtc thread_step eσ1 eσ2 → Wf eσ1.2 → Wf eσ2.2.
+  eσ1 ~t~>* eσ2 → Wf eσ1.2 → Wf eσ2.2.
 Proof.
   intros SS. induction SS; [done|]. intros WF1. apply IHSS. revert WF1.
   by apply thread_step_wf.
 Qed.
 
-Definition sim_expr (sim_thread: SIM_THREAD) (sim_terminal : SIM_EXPR)
-  (e_src e_tgt: expr) : Prop :=
-  ∀ σ_src σ_tgt, sim_thread sim_terminal e_src σ_src e_tgt σ_tgt.
 
-Lemma sim_expr_mono st1 st2 : st1 <5= st2 → sim_expr st1 <3= sim_expr st2.
-Proof. intros ST ??? PR ??. by apply ST, PR. Qed.
+Notation SIM_STATE := (relation state)%type.
+
+Inductive sim_terminal (sim_state : SIM_STATE) : SIM_CONFIG :=
+| SimTerminal e_src σ_src e_tgt σ_tgt
+    (TERM: terminal e_tgt)
+    (VAL: sim_val_expr e_src e_tgt)
+    (STATE: sim_state σ_src σ_tgt)
+  : sim_terminal sim_state (e_src, σ_src) (e_tgt, σ_tgt).
+
+Definition sim_expr (sim_thread: SIM_THREAD)
+  (simp_pre : SIM_STATE) (e_src e_tgt: expr) (sim_post : SIM_STATE) : Prop :=
+  ∀ σ_src σ_tgt, simp_pre σ_src σ_tgt →
+    sim_thread (sim_terminal sim_post) (e_src, σ_src) (e_tgt, σ_tgt).
+
+Lemma sim_expr_mono st1 st2 : st1 <3= st2 → sim_expr st1 <4= sim_expr st2.
+Proof. intros ST ???? PR ???. by apply ST, PR. Qed.
 
 Inductive ctx (sim_thread : SIM_THREAD) : SIM_THREAD :=
-| CtxIncl (sim_terminal : SIM_EXPR) e_src e_tgt σ_src σ_tgt
-    (SIM: sim_thread sim_terminal e_src σ_src e_tgt σ_tgt):
-    ctx sim_thread sim_terminal e_src σ_src e_tgt σ_tgt
-| CtxBinOp (sim_terminal : SIM_EXPR)
+| CtxIncl (sim_post : SIM_CONFIG) eσ_src eσ_tgt
+    (SIM: sim_thread sim_post eσ_src eσ_tgt) :
+    ctx sim_thread sim_post eσ_src eσ_tgt
+| CtxTerm (sim_post : SIM_STATE) eσ_src eσ_tgt
+    (SIM: sim_terminal sim_post eσ_src eσ_tgt) :
+    ctx sim_thread (sim_terminal sim_post) eσ_src eσ_tgt
+| CtxBinOp (sim1 sim2 : SIM_STATE)
+    op e1_src e1_tgt σ1_src σ1_tgt e2_src e2_tgt
+    (SIM1: sim_thread (sim_terminal sim1) (e1_src, σ1_src) (e1_tgt, σ1_tgt))
+    (SIM2: sim_expr sim_thread sim1 e2_src e2_tgt sim2) :
+    ctx sim_thread (sim_terminal sim2) (BinOp op e1_src e2_src, σ1_src)
+                                        (BinOp op e1_tgt e2_tgt, σ1_tgt)
+| CtxBinOpR (sim : SIM_STATE)
     op e1_src e1_tgt σ_src σ_tgt e2_src e2_tgt
-    (SIM1: sim_thread sim_terminal e1_src σ_src e1_tgt σ_tgt)
-    (SIM2: sim_expr sim_thread sim_terminal e2_src e2_tgt) :
-    ctx sim_thread sim_terminal (BinOp op e1_src e2_src) σ_src
-                                (BinOp op e1_tgt e2_tgt) σ_tgt
-| CtxApp (sim_terminal : SIM_EXPR)
+    (TERM1: terminal e1_src) (TERM2: terminal e1_tgt)
+    (SIM1: sim_thread (sim_terminal sim) (e2_src, σ_src) (e2_tgt, σ_tgt)) :
+    ctx sim_thread (sim_terminal sim)
+                   (BinOp op e1_src e2_src, σ_src)
+                   (BinOp op e1_tgt e2_tgt, σ_tgt).
+
+(* | CtxApp (simλ : SIM_STATE)
     e_src e_tgt σ_src σ_tgt el_src el_tgt
-    (SIMF: sim_thread sim_terminal e_src σ_src e_tgt σ_tgt)
+    (SIMF: sim_thread simλ e_src σ_src e_tgt σ_tgt)
     (EQL: length el_src = length el_tgt)
     (SIML: ∀ i ei_tgt, el_tgt !! i = Some ei_tgt →
-      ∃ ei_src, el_src !! i = Some ei_src ∧ 
+      ∃ ei_src, el_src !! i = Some ei_src ∧
       sim_expr sim_thread sim_terminal ei_src ei_tgt) :
     ctx sim_thread sim_terminal (App e_src el_src) σ_src
-                                (App e_tgt el_tgt) σ_tgt
-| CtxProj (sim_terminal : SIM_EXPR)
+                                (App e_tgt el_tgt) σ_tgt. *)
+(* | CtxTVal
+    ctx sim_thread sim_terminal (TVal el_src) σ_src
+                                (TVal el_tgt) σ_tgt. *)
+(* | CtxProj (sim1 sim2 : SIM_STATE)
     e1_src e1_tgt σ_src σ_tgt e2_src e2_tgt
-    (SIM1: sim_thread sim_terminal e1_src σ_src e1_tgt σ_tgt)
-    (SIM2: sim_expr sim_thread sim_terminal e2_src e2_tgt) :
-    ctx sim_thread sim_terminal (Proj e1_src e2_src) σ_src
-                                (Proj e1_tgt e2_tgt) σ_tgt
-| CtxConc (sim_terminal : SIM_EXPR)
+    (SIM1: sim_thread sim1 e1_src σ_src e1_tgt σ_tgt)
+    (SIM2: sim_expr sim_thread sim1 e2_src e2_tgt sim2) :
+    ctx sim_thread sim2 (Proj e1_src e2_src) σ_src
+                        (Proj e1_tgt e2_tgt) σ_tgt
+| CtxConc (sim1 sim2 : SIM_STATE)
     e1_src e1_tgt σ_src σ_tgt e2_src e2_tgt
-    (SIM1: sim_thread sim_terminal e1_src σ_src e1_tgt σ_tgt)
-    (SIM2: sim_expr sim_thread sim_terminal e2_src e2_tgt) :
-    ctx sim_thread sim_terminal (Conc e1_src e2_src) σ_src
-                                (Conc e1_tgt e2_tgt) σ_tgt
-| CtxCopy (sim_terminal : SIM_EXPR)
+    (SIM1: sim_thread sim1 e1_src σ_src e1_tgt σ_tgt)
+    (SIM2: sim_expr sim_thread sim1 e2_src e2_tgt sim2) :
+    ctx sim_thread sim2 (Conc e1_src e2_src) σ_src
+                        (Conc e1_tgt e2_tgt) σ_tgt
+| CtxCopy (sim_post : SIM_STATE)
     e_src e_tgt σ_src σ_tgt
-    (SIM: sim_thread sim_terminal e_src σ_src e_tgt σ_tgt) :
-    ctx sim_thread sim_terminal (Copy e_src) σ_src
+    (SIM: sim_thread sim_post e_src σ_src e_tgt σ_tgt) :
+    ctx sim_thread sim_post (Copy e_src) σ_src
                                 (Copy e_tgt) σ_tgt
-| CtxWrite (sim_terminal : SIM_EXPR)
+| CtxWrite (sim1 sim2 : SIM_STATE)
     e1_src e1_tgt σ_src σ_tgt e2_src e2_tgt
-    (SIM1: sim_thread sim_terminal e1_src σ_src e1_tgt σ_tgt)
-    (SIM2: sim_expr sim_thread sim_terminal e2_src e2_tgt) :
-    ctx sim_thread sim_terminal (Write e1_src e2_src) σ_src
-                                (Write e1_tgt e2_tgt) σ_tgt
-| CtxDeref (sim_terminal : SIM_EXPR) T
+    (SIM1: sim_thread sim1 e1_src σ_src e1_tgt σ_tgt)
+    (SIM2: sim_expr sim_thread sim1 e2_src e2_tgt sim2) :
+    (* FIXME: not sim2, but sim2 + the effect of the write *)
+    ctx sim_thread sim2 (Write e1_src e2_src) σ_src
+                        (Write e1_tgt e2_tgt) σ_tgt
+| CtxDeref (sim_post : SIM_STATE) T
     e_src e_tgt σ_src σ_tgt
-    (SIM: sim_thread sim_terminal e_src σ_src e_tgt σ_tgt) :
-    ctx sim_thread sim_terminal (Deref e_src T) σ_src
-                                (Deref e_tgt T) σ_tgt
-| CtxRef (sim_terminal : SIM_EXPR)
+    (SIM: sim_thread sim_post e_src σ_src e_tgt σ_tgt) :
+    ctx sim_thread sim_post (Deref e_src T) σ_src
+                            (Deref e_tgt T) σ_tgt
+| CtxRef (sim_post : SIM_STATE)
     e_src e_tgt σ_src σ_tgt
-    (SIM: sim_thread sim_terminal e_src σ_src e_tgt σ_tgt) :
-    ctx sim_thread sim_terminal (Ref e_src) σ_src
+    (SIM: sim_thread sim_post e_src σ_src e_tgt σ_tgt) :
+    ctx sim_thread sim_post (Ref e_src) σ_src
                                 (Ref e_tgt) σ_tgt
-| CtxField (sim_terminal : SIM_EXPR) path
+| CtxField (sim_post : SIM_STATE) path
     e_src e_tgt σ_src σ_tgt
-    (SIM: sim_thread sim_terminal e_src σ_src e_tgt σ_tgt) :
-    ctx sim_thread sim_terminal (Field e_src path) σ_src
-                                (Field e_tgt path) σ_tgt
-| CtxEndCall (sim_terminal : SIM_EXPR)
+    (SIM: sim_thread sim_post e_src σ_src e_tgt σ_tgt) :
+    ctx sim_thread sim_post (Field e_src path) σ_src
+                            (Field e_tgt path) σ_tgt
+| CtxEndCall (sim_post : SIM_STATE)
     e_src e_tgt σ_src σ_tgt
-    (SIM: sim_thread sim_terminal e_src σ_src e_tgt σ_tgt) :
-    ctx sim_thread sim_terminal (EndCall e_src) σ_src
-                                (EndCall e_tgt) σ_tgt
-| CtxRetag (sim_terminal : SIM_EXPR) kind
+    (SIM: sim_thread sim_post e_src σ_src e_tgt σ_tgt) :
+    ctx sim_thread sim_post (EndCall e_src) σ_src
+                            (EndCall e_tgt) σ_tgt
+| CtxRetag (sim1 sim2 : SIM_STATE) kind
     e1_src e1_tgt σ_src σ_tgt e2_src e2_tgt
-    (SIM1: sim_thread sim_terminal e1_src σ_src e1_tgt σ_tgt)
-    (SIM2: sim_expr sim_thread sim_terminal e2_src e2_tgt) :
-    ctx sim_thread sim_terminal (Retag e1_src kind e2_src) σ_src
-                                (Retag e1_tgt kind e2_tgt) σ_tgt
-| CtxCase (sim_terminal : SIM_EXPR)
+    (SIM1: sim_thread sim1 e1_src σ_src e1_tgt σ_tgt)
+    (SIM2: sim_expr sim_thread sim1 e2_src e2_tgt sim2) :
+    (* FIXME: not sim2, but sim2 + the effect of the retag *)
+    ctx sim_thread sim2 (Retag e1_src kind e2_src) σ_src
+                        (Retag e1_tgt kind e2_tgt) σ_tgt. *)
+(* | CtxCase (sim_terminal : SIM_STATE)
     e_src e_tgt σ_src σ_tgt el_src el_tgt
     (SIMF: sim_thread sim_terminal e_src σ_src e_tgt σ_tgt)
     (EQL: length el_src = length el_tgt)
@@ -211,25 +233,25 @@ Inductive ctx (sim_thread : SIM_THREAD) : SIM_THREAD :=
       sim_expr sim_thread sim_terminal ei_src ei_tgt) :
     ctx sim_thread sim_terminal (Case e_src el_src) σ_src
                                 (Case e_tgt el_tgt) σ_tgt
-.
+. *)
 
-Lemma ctx_mono: monotone5 ctx.
+Lemma ctx_mono: monotone3 ctx.
 Proof.
-  intros se e1 σ1 e2 σ2 r r' CTX TS. inversion CTX; subst.
+  intros se [e1 σ1] [e2 σ2] r r' CTX TS. inversion CTX; subst.
   - econstructor 1; auto.
-  - econstructor 2; auto. by eapply sim_expr_mono.
-  - econstructor 3; auto. naive_solver eauto using sim_expr_mono.
-  - econstructor 4; auto. by eapply sim_expr_mono.
-  - econstructor 5; auto. by eapply sim_expr_mono.
-  - econstructor 6; auto.
-  - econstructor 7; auto. by eapply sim_expr_mono.
+  - econstructor 2; auto.
+  - econstructor 3. by eapply TS. by eapply sim_expr_mono.
+  - econstructor 4; auto.
+(*   - econstructor 3. by eapply TS. by eapply sim_expr_mono.
+  - econstructor 4. by eapply TS. by eapply sim_expr_mono.
+  - econstructor 5; auto.
+  - econstructor 6. by eapply TS. by eapply sim_expr_mono.
+  - econstructor 7; auto.
   - econstructor 8; auto.
   - econstructor 9; auto.
   - econstructor 10; auto.
-  - econstructor 11; auto.
-  - econstructor 12; auto. by eapply sim_expr_mono.
-  - econstructor 13; auto. naive_solver eauto using sim_expr_mono.
-Qed.
+  - econstructor 11. by eapply TS. by eapply sim_expr_mono.
+ *)Qed.
 
 (** Compatibility: language constructs preserve thread simulation *)
 
@@ -245,9 +267,9 @@ Ltac inv_head_step :=
   end.
 
 Lemma thread_step_bin_op_left_non_terminal op e1 e2 e' σ σ'
-  (STEP: thread_step (BinOp op e1 e2, σ) (e', σ'))
+  (STEP: (BinOp op e1 e2, σ) ~t~> (e', σ'))
   (NT: ¬ terminal e1):
-  ∃ e1', thread_step (e1, σ) (e1', σ') ∧ e' = BinOp op e1' e2.
+  ∃ e1', (e1, σ) ~t~> (e1', σ') ∧ e' = BinOp op e1' e2.
 Proof.
   inversion_clear STEP; simpl in PRIM.
   inversion_clear PRIM as [??? Eq1 ? HS]. subst.
@@ -263,9 +285,9 @@ Proof.
 Qed.
 
 Lemma thread_step_bin_op_right_non_terminal op e1 e2 e' σ σ'
-  (STEP: thread_step (BinOp op e1 e2, σ) (e', σ'))
+  (STEP: (BinOp op e1 e2, σ) ~t~> (e', σ'))
   (TM: terminal e1) (NT: ¬ terminal e2):
-  ∃ e2', thread_step (e2, σ) (e2', σ') ∧ e' = BinOp op e1 e2'.
+  ∃ e2', (e2, σ) ~t~> (e2', σ') ∧ e' = BinOp op e1 e2'.
 Proof.
   inversion_clear STEP; simpl in PRIM.
   inversion_clear PRIM as [??? Eq1 ? HS]. subst.
@@ -283,49 +305,112 @@ Proof.
 Qed.
 
 
-Lemma ctx_weak_respectful: weak_respectful5 _sim_thread ctx.
+Require Import Coq.Program.Equality.
+Lemma thread_step_bin_op_red_r e1 σ1 e1' σ1' e2 e2' σ2' op:
+  (e1, σ1) ~t~>* (e1', σ1') → terminal e1' →
+  (e2, σ1') ~t~>* (e2', σ2') →
+  (BinOp op e1 e2, σ1) ~t~>* (BinOp op e1' e2', σ2').
+Proof.
+  intros S1 T1 S2.
+  etrans. instantiate (1:= (BinOp op e1' e2, σ1')).
+  - clear S2 T1.
+    dependent induction S1 generalizing e1 σ1 e2; first by constructor.
+    destruct y as [e0 σ0].
+    etrans; last apply IHS1; [|eauto..]. apply rtc_once.
+    clear -H. admit.
+  - clear S1.
+    dependent induction S2 generalizing e2 σ1'; first by constructor.
+    destruct y as [e0 σ0].
+    etrans; last apply IHS2; [|eauto..]. apply rtc_once.
+    clear -H. admit.
+Admitted.
+
+Lemma sim_val_expr_terminal e_src e_tgt :
+  sim_val_expr e_src e_tgt → terminal e_tgt → terminal e_src.
+Proof. move => SIM /expr_terminal_True [? /SIM [? [??]]]. by eexists. Qed.
+Lemma expr_terminal_no_step eσ1 eσ2 :
+  terminal eσ1.1 → ¬ thread_step eσ1 eσ2.
+Proof.
+  destruct eσ1 as [e σ].
+  move => EQ STEP.
+  inversion_clear STEP; simpl in PRIM.
+  inversion_clear PRIM as [??? Eq1 ? HS%val_head_stuck]. subst.
+  apply fill_val in EQ.
+  rewrite /= HS in EQ. by destruct EQ.
+Qed.
+
+Lemma sim_terminal_sim_thread
+  (sim: SIM_THREAD) (sim_post: SIM_STATE) eσ_src eσ_tgt :
+  sim_terminal sim_post eσ_src eσ_tgt →
+  _sim_thread sim (sim_terminal sim_post) eσ_src eσ_tgt.
+Proof.
+  intros SIM WF1 WF2. inversion SIM; subst. split.
+  - intros ?. exists (e_src, σ_src). split; [constructor|]. split; [|done].
+    by eapply sim_val_expr_terminal.
+  - intros ??. exfalso. by eapply expr_terminal_no_step; eauto.
+Qed.
+
+Lemma ctx_weak_respectful: weak_respectful3 _sim_thread ctx.
 Proof.
   econstructor; [by apply ctx_mono|].
-  intros l r LE GF se e1 σ1 e2 σ2 CTX.
+  intros l r LE GF se [e1 σ1] [e2 σ2] CTX.
   destruct CTX;
-    [(* incl *) eapply _sim_thread_mono; eauto; apply rclo5_incl|..];
-    intros WF1 WF2 SS;
+    [(* incl *) eapply _sim_thread_mono; eauto; apply rclo3_incl
+    |(* term *) by apply sim_terminal_sim_thread|..];
+    intros WF1 WF2;
     (split; [intros TERM; exfalso; move : TERM; clear; cbv; naive_solver|]);
-    intros e_tgt' σ_tgt' STEP.
+    intros [eo_tgt σo_tgt] STEP.
   - (* BinOp *)
-    destruct (GF _ _ _ _ _ SIM1 WF1 WF2 SS) as [TT ST].
+    destruct (GF _ _ _ SIM1 WF1 WF2) as [TT ST].
     case (decide (terminal e1_tgt)) as [Te1|NTe1].
-    + destruct (TT Te1) as (e1'_src & σ1'_src & RS & SS' & Te1' & ST').
+    + destruct (TT Te1) as ([e1'_src σ1'_src] & RS & Te1' & ST').
+      inversion ST'; subst.
       (* have ST2:= GF _ _ _ _ _ (SIM2 σ1'_src σ_tgt). *)
-      destruct (GF _ _ _ _ _ (SIM2 σ1'_src σ_tgt) (rtc_thread_step_wf _ _ RS WF1)
-                  WF2 SS') as [TT2 ST2].
+      destruct (GF _ _ _ (SIM2 _ _ STATE) (rtc_thread_step_wf _ _ RS WF1)
+                  WF2) as [TT2 ST2].
       case (decide (terminal e2_tgt)) as [Te2|NTe2].
-      * destruct (TT2 Te2) as (e2'_src & σ2'_src & RS2 & SS2' & Te2' & ST2').
-        admit.
+      * destruct (TT2 Te2) as ([e2'_src σ2'_src] & RS2 & Te2' & ST2').
+        eexists (_, σ2'_src). split.
+        { admit. }
+        { apply rclo3_step, CtxTerm. inversion ST2'; subst. constructor.
+          - admit.
+          - admit.
+          - (* σo_tgt - σ1_tgt *) admit. }
       * destruct (thread_step_bin_op_right_non_terminal _ _ _ _ _ _ STEP Te1 NTe2)
           as [e2'_tgt [STEP' Eq']]. rewrite Eq'.
-        destruct (ST2 _ _ STEP') as (e2'_src & σ2'_src & RS2 & SS2' & HR).
-        exists (BinOp op e1'_src e2'_src), σ2'_src. split; last split; [|done|].
-        { admit. }
-        { apply rclo5_step, CtxBinOp.
-          - apply rclo5_incl. admit.
-          - eapply sim_expr_mono; [by apply rclo5_incl|].
-            eapply sim_expr_mono; [by apply LE|].
-            admit. }
+        destruct (ST2 _ STEP') as ([e2'_src σ2'_src] & TS' & HR).
+        exists (BinOp op e1'_src e2'_src, σ2'_src). split.
+        { eapply thread_step_bin_op_red_r; eauto. }
+        { apply rclo3_step, CtxBinOpR; auto. by apply rclo3_incl. }
     + destruct (thread_step_bin_op_left_non_terminal _ _ _ _ _ _ STEP NTe1)
         as [e1'_tgt [STEP' Eq']]. rewrite Eq'.
-      destruct (ST _ _ STEP') as (e1'_src & σ1'_src & RS & SS' & HR).
-      exists (BinOp op e1'_src e2_src), σ1'_src. split; last split; [|done|].
+      destruct (ST _ STEP') as ([e1'_src σ1'_src] & RS & HR).
+      exists (BinOp op e1'_src e2_src, σ1'_src). split.
       * admit.
-      * apply rclo5_step, CtxBinOp.
-        { by apply rclo5_incl. }
-        { eapply sim_expr_mono; [by apply rclo5_incl|].
+      * eapply rclo3_step, CtxBinOp.
+        { by apply rclo3_incl. }
+        { eapply sim_expr_mono; [by apply rclo3_incl|].
           eapply sim_expr_mono; [by apply LE|done]. }
-  - (* App *) admit.
-  - (* Proj *) admit.
+  - (* BinOpR *)
+    destruct (GF _ _ _ SIM1 WF1 WF2) as [TT ST].
+    case (decide (terminal e2_tgt)) as [Te2|NTe2].
+    + destruct (TT Te2) as ([e2'_src σ2'_src] & RS2 & Te2' & ST2').
+      eexists (_, σ2'_src). split.
+      { admit. }
+      { apply rclo3_step, CtxTerm. inversion ST2'; subst.
+        constructor.
+        - admit.
+        - admit.
+        - (* σo_tgt - σ1_tgt *) admit. }
+    + destruct (thread_step_bin_op_right_non_terminal _ _ _ _ _ _ STEP TERM2 NTe2)
+        as [e2'_tgt [STEP' Eq']]. rewrite Eq'.
+      destruct (ST _ STEP') as ([e2'_src σ2'_src] & TS' & HR).
+      exists (BinOp op e1_src e2'_src, σ2'_src). split.
+      { admit. }
+      { apply rclo3_step, CtxBinOpR; auto. by apply rclo3_incl. }
 Abort.
 
-Lemma ctx_respectful: respectful5 _sim_thread ctx.
+(* Lemma ctx_respectful: respectful5 _sim_thread ctx.
 Proof.
   econstructor; [by apply ctx_mono|].
   intros l r LE M2 se e1 σ1 e2 σ2 CTX.
@@ -362,4 +447,4 @@ Proof.
         { by apply rclo5_incl. }
         { eapply sim_expr_mono; [by apply rclo5_incl|].
           eapply sim_expr_mono; [by apply LE|done]. }
-Abort.
+Abort. *)
